Structures/Blocks.v
@@ -1,0 +1,45 @@
+From mathcomp.ssreflect
+Require Import ssreflect ssrbool ssrnat eqtype ssrfun seq.
+From mathcomp
+Require Import path.
+Require Import Eqdep pred prelude idynamic ordtype pcm finmap unionmap heap coding.
+Require Import SeqFacts Chains.
+Set Implicit Arguments.
+Unset Strict Implicit.
+Unset Printing Implicit Defensive.
+
+Definition Hash := [ordType of nat].
+
+Record Block {Transaction VProof : eqType} :=
+  mkB {
+    height : nat;
+    prevBlockHash : Hash;
+    txs : seq Transaction;
+    proof : VProof;
+  }.
+
+Definition eq_block {T P : eqType} (b b' : @Block T P) :=
+  match (b, b') with
+  | (mkB h p t pf, mkB h' p' t' pf') =>
+    [&& h == h', p == p', t == t' & pf == pf']
+  end.
+      
+Lemma eq_blockP {T P : eqType} : Equality.axiom (@eq_block T P).
+Proof.
+case=> h p t pf; case=> h' p' t' pf'; rewrite /eq_block/=.
+case H1: (h == h'); [move/eqP: H1=>?; subst h'| constructor 2];
+  last by case=>?; subst h';rewrite eqxx in H1.
+case H2: (p == p'); [move/eqP: H2=>?; subst p'| constructor 2];
+  last by case=>?; subst p';rewrite eqxx in H2.
+case H3: (t == t'); [move/eqP: H3=>?; subst t'| constructor 2];
+  last by case=>?; subst t';rewrite eqxx in H3.
+case H4: (pf == pf'); [move/eqP: H4=>?; subst pf'| constructor 2];
+  last by case=>?; subst pf';rewrite eqxx in H4.
+by constructor 1. 
+Qed.
+
+Canonical Block_eqMixin {T P : eqType} :=
+  Eval hnf in EqMixin (@eq_blockP T P).
+Canonical Block_eqType {T P : eqType} :=
+  Eval hnf in EqType (@Block T P) (@Block_eqMixin T P).
+
